new compose alt modulo some admitted shft stuff

theories/VACCScompose/altchar/AltCompose.v
@@ -1,54 +1,6 @@
 
-(*--------------a bunch of imports--------------------*)
-From Stdlib Require Export Program.Equality .
-From TestingTheory Require Export Must VACCS_Good gLts InteractionBetweenLts ActTau.
-Include VACCS_Testing.
 
-
-Require Import DefinitionAS.
-Require Import Convergence.
-Require Import Termination.
-Require Import List.
-Require Import stdpp.base.
-(*Require Import WeakTransitions.*)
- 
-
-Require Import ForwarderConstruction.
-
-
-(*-----temporary ???-----*)
-From stdpp Require Import gmap.
-(*--------------------*)
-(**)
-(*------------------------------------------------------*)
-
-Print FW_gLts.
-
-
-
-Locate MbLts.
-Notation wt := WeakTransitions.wt.
-Notation tau p := (g (𝛕 • p)).  
-Notation inp x p := (g (gpr_input x p)).
-Print wt.
-
-
-Hint Constructors lts :mdb.
-
-
-Notation Linp c v :=  ( ActTau.ActExt (InputOutputActions.ActIn (c ⋉ v)) ).
-Notation Lout c v := ( ActTau.ActExt (InputOutputActions.ActOut (c ⋉ v))  ).
-Notation Ltau := ActTau.τ.
-Notation sub t1 x1 :=  (subst_in_proc 0 x1 t1).
-
-Locate "^".
-
-
-
-
-
-
-
+Require Import AltGenerality.
 
 
 
@@ -138,12 +90,6 @@ inversion Hwt; inversion l; subst.
 eexists; split; eauto.
 Qed.
 
-Lemma mu_impl_wt: forall p q mu, lts p (ActExt mu) q ->  
-  wt p [mu] q.
-Proof.
-intros ? ? ? Hp.  
-eapply WeakTransitions.wt_act; eauto with mdb.
-Qed.
 
 
 Lemma lcnv_comp_inp: forall x p q,
@@ -165,6 +111,8 @@ Qed.
 
 
 
+
+
 Lemma lacc_comp_inp: forall x p q,
  (forall v, sub p v ≼₂ sub q v) ->  inp x p  ≼₂ inp x q. 
 Proof.
@@ -174,7 +122,7 @@ destruct s.
 - exists (inp x p); repeat split; eauto; try constructor.
   inversion Hwt; try inversion l; subst. 
   
-  (**** tentativede preuve 
+  (****  preuve de 
          R(x?(y).p)⊆R(x?(y).q )*****)
    clear  Hwt Href Hcnv Hplq.
    intro. intro. 
@@ -182,14 +130,20 @@ destruct s.
    exists mu.  
    split. 
    + destruct G1 as [mu0 [G1 [G2 G3]]].
-     exists mu0; repeat split; eauto.
-     intro. inversion H.  
-     destruct mu0, (decide (ChannelData_of a = x)).
-     * inversion H1.
-     * admit.
-     * admit.
-     * admit.
-   + unfold 𝝳ᴠᴀᴄᴄꜱ, "∘", Φᴠᴀᴄᴄꜱ.
+     unfold "blocking", non_blocking in *.
+     (*cbn in *.*)
+     unfold non_blocking_output, InputOutputActions.is_output in *.
+     destruct (inv_mu mu) as  [c [v inv_mu]].
+     destruct inv_mu as [inv_mu|inv_mu].
+     * inversion inv_mu; subst. clear inv_mu.
+       destruct (inv_mu mu0) as  [c0 [v0 inv_mu0]].
+       destruct inv_mu0 as [inv_mu0|inv_mu0]; subst.
+       inversion inv_mu0; subst; cbv in G2; try (exfalso; auto).
+       inversion inv_mu0; subst; cbv in G2; inversion G2; subst.
+       set_solver.
+     * exfalso; apply G3.
+       exists (act c v); inversion inv_mu; auto.
+    + unfold 𝝳ᴠᴀᴄᴄꜱ, "∘", Φᴠᴀᴄᴄꜱ.
      destruct mu,a; auto.      
   (*********)
 - set (lem:= wt_inp _ _ _ _ _ Hwt).
@@ -205,7 +159,7 @@ destruct s.
   destruct Hplq as[P[Hwtp [HPref Hsubset]]].
   exists P; repeat split; eauto.
   eapply WeakTransitions.wt_act; try constructor; eauto.
-Admitted.
+Qed.
 
 
 Proposition alt_comp_inp: forall x p q,
@@ -216,171 +170,13 @@ try eapply lcnv_comp_inp; try eapply lacc_comp_inp; apply Hplq.
 Qed.
 
 
-(*==================  Nu  =============================*)
-
-Notation ash mu :=  (VarC_action_add 1 mu).
-
-(*shift on trace*)
-Fixpoint sh s := match s with
-  | nil   => nil
-  | mu::s' => (ash mu):: sh s'  
-end.
-
-
-
-Lemma shift_nil: forall s, nil=sh s -> s=nil.
-Proof. 
-intros ? H; destruct s; auto.
-cbn in H; inversion H.
-Qed.
-
-Lemma shift_cons: forall mu s s', mu::s'=sh s -> 
-  exists mu0 s0, s=mu0::s0 /\ 
-  mu= ash mu0 /\ s'=sh s0.
-Proof.
-intros ? ? ? H; destruct s; cbn in *; 
-inversion H; eauto.
-Qed.
-
-
-Lemma wt_unshift: forall p q s, wt p (sh s) q -> 
-  wt (ν p) s (ν q).  
-Proof.
-intros ? ? ? Hwt.
-dependent induction Hwt.
-- apply shift_nil in x; subst; constructor.
-- specialize (IHHwt s JMeq_refl);  
-  eapply WeakTransitions.wt_tau;  
-  try constructor; eauto. 
-- apply shift_cons in x.
-  destruct x as [mu0[s1[Heqs[Heqmu Heqs0]]]]; subst.
-  specialize (IHHwt _ JMeq_refl).  
-  eapply WeakTransitions.wt_act; 
-  try constructor; eauto.
-Qed.
-
-
-Lemma wt_unshiftmu: forall p q mu, wt p [ash mu] q -> 
-  wt (ν p) [mu] (ν q).  
-Proof.
-eauto using wt_unshift.
-Qed.
-
-
-Lemma wt_shift: forall p Q s, wt (ν p) s Q -> 
-  exists p', wt p (sh s)  p' /\ Q=ν p'.
-Proof.
-intros ? ? ? Hwt.
-dependent induction Hwt; eauto with mdb. 
-- inversion l; subst. 
-  specialize (IHHwt _ eq_refl). 
-  destruct IHHwt as [p''[Hwtp' Heq]]. 
-  eauto with mdb.
-- inversion l; subst.
-  specialize (IHHwt _ eq_refl).
-  destruct IHHwt as [p''[Hwtp' Heq]]; subst. 
-  exists p''; split; 
-  try eapply WeakTransitions.wt_act; eauto.
-Qed.
-
-Lemma wt_shiftmu: forall p Q mu, wt (ν p) [mu] Q -> 
-  exists p', wt p [ash mu]  p' /\ Q=ν p'.
-Proof. 
-intros ? ? ? H.
-eauto using (wt_shift _ _ _ H).
-Qed.
-
-
-
-Lemma term_nu: forall p, (ν p)⤓ -> p⤓.
-Proof.
-intros ? Hter; dependent induction Hter. 
-constructor; intros p' Hp.
-eapply H0; constructor; eauto.
-Qed.
-
-Lemma term_nu_rev: forall p, p⤓ -> (ν p)⤓.
-Proof.
-intros ? Hter; dependent induction Hter.
-constructor; intros P Hnup; inversion Hnup.
-eauto with mdb.
-Qed.
-
-
-
-
-
-
-Lemma cnv_nu: forall s p,
-  (ν p)⇓s -> p⇓(sh s) .
-Proof.
-intros ? ?; generalize dependent p. 
-induction s; intros ? Hcnv; 
-inversion Hcnv; subst; cbn in *; 
-try (constructor; auto using term_nu). 
-intros p' Hwt; inversion Hwt; subst.
-- eapply wt_unshiftmu in w.
-  eapply IHs, H3, wt_unshiftmu; auto.
-- apply lts_res_ext, mu_impl_wt in l.
-  specialize (H3 _ l); specialize (IHs _ H3).
-  eapply cnv_preserved_by_wt_nil; eauto.
-Qed.
-
-Lemma cnv_nu_rev: forall s p,
-  p⇓(sh s) -> (ν p)⇓s.
-Proof.
-intros ? ? Hcnv.
-dependent induction Hcnv.
-- apply shift_nil in x; subst; constructor;
-  auto using term_nu_rev.
-- apply shift_cons in x; subst.
-  destruct x as [mu0 [s1 [Heqs [Heqmu Heqs0]]]]; subst.
-  constructor; auto using term_nu_rev.
-  intros P Hwt; apply wt_shiftmu in Hwt.
-  destruct Hwt as [p' [Hwt Heq]]; subst; eauto.
-Qed.
-
-
-Lemma lcnv_comp_nu: forall p q,
-  p ≼₁ q ->  (ν p)  ≼₁ (ν q) . 
-Proof.
-unfold "≼₁"; intros ? ? Hplq ? Htaup.
-eapply cnv_nu_rev, Hplq, cnv_nu; auto.
-Qed.
-
-
-
-Lemma lacc_comp_nu: forall p q,
-  p ≼₂ q ->  (ν p)  ≼₂ (ν q) . 
-Proof.
-intros ? ? Hplq; unfold "≼₂".
-intros ? Q Hcnv Hwt Href.
-apply wt_shift in Hwt.
-apply cnv_nu in Hcnv.
-unfold "≼₂" in Hplq.
-destruct Hwt as [q'[Hwt Heq]]; subst.
-specialize (Hplq _ _ Hcnv Hwt).
-assert (q' ↛). set_solver.
-specialize (Hplq H).
-destruct Hplq as [p0 [Hwtp [Hrefp0 Hsubset]]]; subst.
-exists (ν p0); repeat split.
-- apply wt_unshift, Hwtp.
-- set_solver.
-- intro. intro. 
-  destruct H0 as [mu [G1 G2]].
-  assert (mu ∈ Subset_Act.coR p0).
-  unfold Subset_Act.coR in *.
-  destruct G1 as [mu0 [K1 [K2 K3]]]. 
-  eexists; repeat split; eauto. 
-  intro. apply K1. 
-  admit.
-  econstructor; split; eauto.
-  admit.
-Admitted.
-
-
-
 (*=================   sum   ======================*)
+
+
+
+
+
+
 
 Notation sum p q := (gpr_choice p q).
 
@@ -492,5 +288,18 @@ unfold "≼₁"; intros ? ? Hplq ? Hsum.
 apply cnv_sum in Hsum; destruct Hsum; 
 apply cnv_sum_rev; auto.
 Qed.
+
+
+
+
+(*
+Lemma blah: forall p a,
+  lts_set p a ≠ ∅ -> exists p', lts p a p'.
+Proof.
+intros.
+destruct a.
+Focus 2.
+cbn in H.
+*)
 
 
