theories/VACCScompose/altchar/AltComposeNu.v
@@ -1,0 +1,303 @@
+
+
+
+Require Import AltGenerality.
+
+
+
+
+
+
+
+
+
+
+
+
+
+
+
+
+
+Notation ash mu :=  (VarC_action_add 1 mu). (*ash=action shift*)
+Notation alpha := (𝝳ᴠᴀᴄᴄꜱ ∘ Φᴠᴀᴄᴄꜱ). (*abstraction on a mu*)
+Notation Alpha := (Subset_Act.map_set alpha). (*abstraction on a set of mus*)
+
+
+(*shift on trace*)
+Fixpoint sh s := match s with
+  | nil   => nil
+  | mu::s' => (ash mu):: sh s'  
+end.
+
+
+
+
+
+
+
+(*================ admitted stuff ================================*)
+Lemma dual_shift: forall mu1 mu2,
+  dual mu1 mu2 ->
+  dual (ash mu1) (ash mu2).
+Proof. Admitted.
+
+Lemma blocking_shift: forall mu,
+  blocking mu -> blocking (ash mu).
+Proof. Admitted. 
+
+Lemma blocking_shift_rev: forall mu,
+  blocking (ash mu) -> blocking mu.
+Proof. Admitted. 
+
+
+Lemma shift_procstable_inv: forall p mu, 
+  proc_stable p (ActExt (ash mu)) ->
+  proc_stable p (ActExt mu) .
+Proof. Admitted. 
+
+
+Lemma dual_shift_inv: forall mu1 mu2, dual mu1 (ash mu2) ->
+  exists mu0, mu1 = ash mu0 /\ dual mu0 mu2.
+Proof. Admitted.
+
+Lemma inv_alpha: forall mu1 mu2,
+  alpha (ash mu1) = alpha mu2 -> 
+  exists mu0, mu2 = ash mu0 /\ alpha mu1 = alpha mu0 .
+Proof. Admitted. 
+ 
+(*=========================================================*)
+
+
+(*-----------misc----------------------*)
+Lemma inv_nonmublock_precise: forall p mu,
+  (¬ (p ↛[mu])) -> exists x v q,
+  
+  ((ActExt mu) =  Linp x v /\ lts p (Linp x v) q)  \/ 
+  ((ActExt mu) =  Lout x v /\lts p (Lout x v) q) .
+Proof.
+intros ? ? Hnmb.
+simpl in Hnmb.
+unfold proc_stable, lts_set in *.
+destruct (inv_mu mu) as [x [v H]].
+destruct H as [H|H]; inversion H; subst; eauto.
+- set (empdec:=  set_choose_or_empty (lts_set_input p (x ⋉ v))) .
+  destruct empdec as [empdec|empdec].
+  * destruct empdec as [q empdec]. set (lem:= lts_set_input_spec0 _ _ _ empdec).
+     repeat eexists; eauto.
+  * set_solver.
+- set (empdec:=  set_choose_or_empty (lts_set_output p (x ⋉ v))) .
+  destruct empdec as [empdec|empdec].
+  * destruct empdec as [q empdec]. set (lem:= lts_set_output_spec0 _ _ _ empdec).
+     repeat eexists; eauto.
+  * set_solver.
+Qed.
+
+
+Lemma inv_nonmublock: forall p mu,
+  (¬ (p ↛[mu])) -> exists q, lts p (ActExt mu) q  .
+Proof.
+intros ? ? H. set (lem:= inv_nonmublock_precise _ _ H).
+destruct lem as [x [c [q [[Heq lem]|[Heq lem]]]]]; rewrite Heq; eauto.
+Qed.
+
+
+Lemma inv_nonmublock_rev: forall p mu,
+  (exists q, lts p (ActExt mu) q)  -> (¬ (p ↛[mu]))  .
+Proof.
+intros ? ? H. 
+destruct H as [q Hlt].
+intro.
+set (lem := inv_mu mu).
+destruct lem as [x [v [Hmueq|Hmueq]]]; inversion Hmueq; subst.
+- eapply lts_set_input_spec1 in Hlt; set_solver.
+- eapply lts_set_output_spec1 in Hlt; set_solver.
+Qed.
+
+Lemma nonref_nu: forall p mu, 
+  ¬ (ν p) ↛[mu]  ->  ¬ p ↛[ash mu] .
+Proof.
+intros ? ? H. 
+set (lem:= inv_nonmublock _ _ H).
+destruct lem as [q Hlt].
+inversion Hlt; subst.
+eauto using inv_nonmublock_rev.
+Qed.
+
+Lemma nonref_nu_rev: forall p mu, 
+  ¬ p ↛[ash mu] -> ¬ (ν p) ↛[mu].
+Proof.
+intros ? ? H. 
+set (lem:= inv_nonmublock _ _ H).
+destruct lem as [q Hlt]. 
+apply lts_res_ext in Hlt.
+eauto using inv_nonmublock_rev.
+Qed.
+
+
+
+(*----------------trace------------------------*)
+Lemma shift_nil: forall s, nil=sh s -> s=nil.
+Proof. 
+intros ? H; destruct s; auto.
+cbn in H; inversion H.
+Qed.
+
+Lemma shift_cons: forall mu s s', mu::s'=sh s -> 
+  exists mu0 s0, s=mu0::s0 /\ 
+  mu= ash mu0 /\ s'=sh s0.
+Proof.
+intros ? ? ? H; destruct s; cbn in *; 
+inversion H; eauto.
+Qed.
+(*----------weak transitions ------------------*)
+
+Lemma wt_unshift: forall p q s, wt p (sh s) q -> 
+  wt (ν p) s (ν q).  
+Proof.
+intros ? ? ? Hwt.
+dependent induction Hwt.
+- apply shift_nil in x; subst; constructor.
+- specialize (IHHwt s JMeq_refl);  
+  eapply WeakTransitions.wt_tau;  
+  try constructor; eauto. 
+- apply shift_cons in x.
+  destruct x as [mu0[s1[Heqs[Heqmu Heqs0]]]]; subst.
+  specialize (IHHwt _ JMeq_refl).  
+  eapply WeakTransitions.wt_act; 
+  try constructor; eauto.
+Qed.
+
+
+Lemma wt_unshiftmu: forall p q mu, wt p [ash mu] q -> 
+  wt (ν p) [mu] (ν q).  
+Proof.
+eauto using wt_unshift.
+Qed.
+
+
+Lemma wt_shift: forall p Q s, wt (ν p) s Q -> 
+  exists p', wt p (sh s)  p' /\ Q=ν p'.
+Proof.
+intros ? ? ? Hwt.
+dependent induction Hwt; eauto with mdb. 
+- inversion l; subst. 
+  specialize (IHHwt _ eq_refl). 
+  destruct IHHwt as [p''[Hwtp' Heq]]. 
+  eauto with mdb.
+- inversion l; subst.
+  specialize (IHHwt _ eq_refl).
+  destruct IHHwt as [p''[Hwtp' Heq]]; subst. 
+  exists p''; split; 
+  try eapply WeakTransitions.wt_act; eauto.
+Qed.
+
+Lemma wt_shiftmu: forall p Q mu, wt (ν p) [mu] Q -> 
+  exists p', wt p [ash mu]  p' /\ Q=ν p'.
+Proof. 
+intros ? ? ? H.
+eauto using (wt_shift _ _ _ H).
+Qed.
+(*------------ convergence -----------------*)
+
+
+Lemma term_nu: forall p, (ν p)⤓ -> p⤓.
+Proof.
+intros ? Hter; dependent induction Hter. 
+constructor; intros p' Hp.
+eapply H0; constructor; eauto.
+Qed.
+
+Lemma term_nu_rev: forall p, p⤓ -> (ν p)⤓.
+Proof.
+intros ? Hter; dependent induction Hter.
+constructor; intros P Hnup; inversion Hnup.
+eauto with mdb.
+Qed.
+
+Lemma cnv_nu: forall s p,
+  (ν p)⇓s -> p⇓(sh s) .
+Proof.
+intros ? ?; generalize dependent p. 
+induction s; intros ? Hcnv; 
+inversion Hcnv; subst; cbn in *; 
+try (constructor; auto using term_nu). 
+intros p' Hwt; inversion Hwt; subst.
+- eapply wt_unshiftmu in w.
+  eapply IHs, H3, wt_unshiftmu; auto.
+- apply lts_res_ext, mu_impl_wt in l.
+  specialize (H3 _ l); specialize (IHs _ H3).
+  eapply cnv_preserved_by_wt_nil; eauto.
+Qed.
+
+Lemma cnv_nu_rev: forall s p,
+  p⇓(sh s) -> (ν p)⇓s.
+Proof.
+intros ? ? Hcnv.
+dependent induction Hcnv.
+- apply shift_nil in x; subst; constructor;
+  auto using term_nu_rev.
+- apply shift_cons in x; subst.
+  destruct x as [mu0 [s1 [Heqs [Heqmu Heqs0]]]]; subst.
+  constructor; auto using term_nu_rev.
+  intros P Hwt; apply wt_shiftmu in Hwt.
+  destruct Hwt as [p' [Hwt Heq]]; subst; eauto.
+Qed.
+
+(*-------------- composition --------------*)
+
+Lemma lcnv_comp_nu: forall p q,
+  p ≼₁ q ->  (ν p)  ≼₁ (ν q) . 
+Proof.
+unfold "≼₁"; intros ? ? Hplq ? Htaup.
+eapply cnv_nu_rev, Hplq, cnv_nu; auto.
+Qed.
+
+
+
+
+Lemma lacc_comp_nu: forall p q,
+  p ≼₂ q ->  (ν p)  ≼₂ (ν q) . 
+Proof.
+intros ? ? Hplq; unfold "≼₂".
+intros ? Q Hcnv Hwt Href.
+apply wt_shift in Hwt.
+apply cnv_nu in Hcnv.
+unfold "≼₂" in Hplq.
+destruct Hwt as [q'[Hwt Heq]]; subst.
+specialize (Hplq _ _ Hcnv Hwt).
+assert (q' ↛). set_solver.
+specialize (Hplq H).
+destruct Hplq as [p0 [Hwtp [Hrefp0 Hsubset]]]; subst.
+exists (ν p0); repeat split.
+- apply wt_unshift, Hwtp.
+- set_solver.
+
+(*=============== ready set inclusion =================*)
+- intro. intro.
+  destruct H0 as [mu [G1 G2]].
+  destruct G1 as [mu0 [F1 [F2 F3]]].
+  
+    (*---------assertion1---------------*) 
+    assert( (alpha (ash mu))∈ Alpha (Subset_Act.coR p0)).  
+   eexists; split; eauto.
+     apply dual_shift in F2; apply blocking_shift in F3.
+     exists (ash mu0); repeat split; auto.
+     auto using nonref_nu.
+   (*----------assertion2-----------------------*)
+    assert (alpha (ash mu)
+    ∈ Alpha (Subset_Act.coR q')).
+    set_solver.
+   (*---------------------------------*)
+    clear Hwtp Hrefp0 Hcnv Hwt Href H. 
+    clear H0.
+    destruct H1 as [mu1 [T D]]; destruct T as [mu2 [T1 [T2 T3]]].
+    apply inv_alpha in D; destruct D as [mu3 [Heq1 Heqalph]]; subst.
+    apply dual_shift_inv in T2; destruct T2 as [mu4 [S1 S2]]; subst.
+    eexists; split; eauto.  
+    eexists; repeat split; eauto using nonref_nu_rev. 
+    apply blocking_shift_rev; auto.
+(*====================================================*)
+Qed.
+
+ 
