theories/VACCScompose/altchar/AltComposePar.v
@@ -1,0 +1,109 @@
+
+
+Require Import AltGenerality.
+
+
+
+
+
+
+(*------------weak transitions -------------*)
+Lemma wt_parL: forall p p' q s, 
+  wt p s p' -> wt (p ‖ q) s (p' ‖ q).
+Proof.
+intros ? ? ? ? Hwt.
+dependent induction Hwt; eauto with mdb.
+- eapply WeakTransitions.wt_tau; try eapply lts_parL; eauto.
+- eapply WeakTransitions.wt_act; try eapply lts_parL; eauto.
+Qed.
+
+Lemma wt_parR: forall p q q' s, 
+  wt q s q' -> wt (p ‖ q) s (p ‖ q').
+Proof.
+intros ? ? ? ? Hwt.
+dependent induction Hwt; eauto with mdb.
+- eapply WeakTransitions.wt_tau; try eapply lts_parR; eauto.
+- eapply WeakTransitions.wt_act; try eapply lts_parR; eauto.
+Qed.
+(*-------------- convergence ------------------*)
+Lemma term_parL: forall p q,  (p‖q)⤓ -> p⤓ .
+Proof.
+intros ? ? H.
+dependent induction H; constructor.
+intros p' Hp.
+eapply H0; constructor; auto.
+Qed.
+
+Lemma term_parR: forall p q,  (p‖q)⤓ -> q⤓ .
+Proof.
+intros ? ? H.
+dependent induction H; constructor.
+intros p' Hp.
+eapply H0; constructor; auto.
+Qed.
+
+Lemma cnv_parL: forall p q s, (p‖q)⇓s ->  p⇓s.
+Proof.
+intros ? ? ? Hcnv.
+dependent induction Hcnv; constructor; eauto using term_parL.
+intros p' Hwt.
+eapply H1; eauto with mdb.
+eauto using wt_parL.
+Qed.
+
+Lemma cnv_parR: forall p q s, (p‖q)⇓s ->  q⇓s.
+Proof.
+intros ? ? ? Hcnv.
+dependent induction Hcnv; constructor; eauto using term_parR.
+intros q' Hwt.
+eapply H1; eauto with mdb.
+eauto using wt_parR.
+Qed.
+(*-------------------------------------------*)
+
+(* gtrace= generalized trace *)
+CoInductive gtrace {A:Type} :=
+| gnil
+| gcons (x:A) (xs:gtrace)  .
+
+(* vact= visible action *)
+Notation vact := (InputOutputActions.ExtAct TypeOfActions).
+Notation "x :: xs" := (gcons x xs).        
+Notation "[]" := gnil.        
+
+
+(* tts= trace transition system *)
+CoInductive tts: proc -> gtrace -> Prop :=
+| tts_nil: forall p, tts p gnil
+| tts_cons: forall p p' mu s, 
+    lts p mu p' -> tts p' s -> tts p' (mu::s). 
+
+CoInductive zip: gtrace -> gtrace -> gtrace -> Prop :=
+| zip_nil: zip [] [] []
+| zip_consL: forall s s1 s2 mu,
+    zip s s1 s2 -> zip (mu::s) (mu::s1) s2 
+| zip_consR: forall s s1 s2 mu,
+    zip s s1 s2 -> zip (mu::s) s1 (mu::s2) 
+| zip_consLR: forall s s1 s2 mu1 mu2,
+    zip s s1 s2 -> dual mu1 mu2 -> 
+    zip s (mu1::s1) (mu2::s2) 
+.
+
+(*
+(* basically the definition of cnv but declared as coinductive*)
+CoInductive gcnv: proc -> gtrace -> Prop :=
+| cnv_nil : forall p,  p ⤓ -> gcnv p []
+| cnv_act : forall p mu s,
+    p ⤓ -> (forall q, wt p [mu] q -> gcnv q s) -> 
+    gcnv p (mu::s).
+Notation "p ⇓ s" := (cocnv p s).
+*)
+Hint Constructors  zip tts gtrace: mdb.
+
+
+Lemma cocnv_parL: forall p q (s:gtrace), (p‖q)⇓s -> p⇓s.
+Proof.
+intros ? ? ? Hcocnv.
+
+
+
