theories/VACCScompose/altchar/AltGenerality.v
@@ -1,0 +1,48 @@
+
+
+(*--------------a bunch of imports--------------------*)
+From Stdlib Require Export Program.Equality .
+From stdpp Require Export gmap.
+From TestingTheory Require Export Must VACCS_Good gLts InteractionBetweenLts ActTau.
+Include VACCS_Testing.
+
+
+From TestingTheory Require Export DefinitionAS Convergence Termination.
+
+Require Export List.
+Require Export stdpp.base.
+ 
+
+Require Export ForwarderConstruction.
+(*---------------- notations -------------------------*)
+Notation wt := WeakTransitions.wt.
+Notation tau p := (g (𝛕 • p)).  
+Notation inp x p := (g (gpr_input x p)).
+
+Notation Linp c v :=  ( ActTau.ActExt (InputOutputActions.ActIn (c ⋉ v)) ).
+Notation Lout c v := ( ActTau.ActExt (InputOutputActions.ActOut (c ⋉ v))  ).
+Notation Ltau := ActTau.τ.
+Notation sub t1 x1 :=  (subst_in_proc 0 x1 t1).
+
+(*---------------------------------------------------*)
+
+
+Hint Constructors lts :mdb.
+
+
+
+Lemma inv_mu: forall mu:InputOutputActions.ExtAct TypeOfActions,
+  exists x v, ( ActExt mu = Linp x v) \/  
+              (ActExt mu = Lout x v)   .
+Proof.
+intros; destruct mu,a; eauto.
+Qed.
+
+
+
+Lemma mu_impl_wt: forall p q mu, lts p (ActExt mu) q ->  
+  wt p [mu] q.
+Proof.
+intros ? ? ? Hp.  
+eapply WeakTransitions.wt_act; eauto with mdb.
+Qed.
